Complete memcpy interop with buffers of UInt64

src/test/interop/memcpy/Memcpy.fst
@@ -6,20 +6,20 @@ module HS = FStar.Monotonic.HyperStack
 
 open Vale_Sem
 open Machine_int
-open Interop
+open Interop64
 module B = FStar.Buffer
 
-let bytes = buffer UInt8.t
+let buf = buffer UInt64.t
 
-let pre_cond (h:HS.mem) (src:bytes) (dest:bytes) =
+let pre_cond (h:HS.mem) (src:buf) (dest:buf) =
   live h src /\ live h dest /\ disjoint src dest /\ length src == 1 /\ length dest == 1
 
-let post_cond (h:HS.mem) (h':HS.mem) (src:bytes) (dest:bytes) =
+let post_cond (h:HS.mem) (h':HS.mem) (src:buf) (dest:buf) =
   live h src /\ live h dest /\ live h' src /\ live h' dest /\ disjoint src dest /\ length src == 1 /\ length dest == 1
     /\ Seq.equal (as_seq h src) (as_seq h' dest)
 
 // Ideally, memcpy would have this form, but we cannot compose STATE and GHOST
-assume val memcpy: src:bytes -> dest:bytes ->
+assume val memcpy: src:buf -> dest:buf ->
   STL unit
     (requires (fun h -> pre_cond h src dest))
     (ensures (fun h0 _ h1 -> post_cond h0 h1 src dest))
@@ -32,47 +32,50 @@ let memcpy_code2 = Mov (OMem (MReg Rbx 0)) (OReg Rax)
 
 #set-options "--z3rlimit 60"
 
-let memcpy_vale (s:state) : (s':state{s.mem.[eval_reg Rax s] == s'.mem.[eval_reg Rbx s]}) = eval_ins memcpy_code2 (eval_ins memcpy_code1 s)
+let memcpy_vale (s:state{s.ok}) : (s':state{get_heap_value (eval_reg Rax s) s == get_heap_value (eval_reg Rbx s) s' /\ s'.ok}) = eval_ins memcpy_code2 (eval_ins memcpy_code1 s)
 
-let pre_v (s:state) (src:bytes) (dst:bytes{disjoint src dst}) (m:HS.mem{live m src /\ live m dst}) = 
+let pre_v (s:state) (src:buf) (dst:buf{disjoint src dst}) (m:HS.mem{live m src /\ live m dst}) = 
   let buffers = [src; dst] in
-  pre_cond (up_mem s.mem addrs buffers m) src dst
+  pre_cond (up_mem64 s.mem addrs buffers m) src dst
   
-let post_v (s1:state) (s2:state) (src:bytes) (dst:bytes{disjoint src dst}) (m:HS.mem{live m src /\ live m dst}) = 
+let post_v (s1:state) (s2:state) (src:buf) (dst:buf{disjoint src dst}) (m:HS.mem{live m src /\ live m dst}) = 
   let buffers = [src; dst] in
-  post_cond (up_mem s1.mem addrs buffers m) (up_mem s2.mem addrs buffers m) src dst
+  s2.ok /\
+  post_cond (up_mem64 s1.mem addrs buffers m) (up_mem64 s2.mem addrs buffers m) src dst
 
-let correct_memcpy (s:state) (src:bytes) (dst:bytes{disjoint src dst}) 
+#set-options "--z3rlimit 200 --initial_fuel 2 --initial_ifuel 1"
+
+let correct_memcpy (s:state{s.ok}) (src:buf) (dst:buf{disjoint src dst}) 
   (m:HS.mem{live m src /\ live m dst}) : Lemma
   (requires (pre_v s src dst m) /\ addrs.[(as_addr src, idx src, length src)] = eval_reg Rax s /\ addrs.[(as_addr dst, idx dst, length dst)] == eval_reg Rbx s)
   (ensures (let s' = memcpy_vale s in post_v s s' src dst m)) =
   let s' = memcpy_vale s in
-  let buffers = [src; dst] in
-  up_mem_liveness s.mem s'.mem addrs buffers m;
+  let (buffers: list (buffer UInt64.t){list_live m buffers /\ list_disjoint_or_eq buffers}) = [src; dst] in
+  up_mem_liveness64 s.mem s'.mem addrs buffers m;
   ()
 
 // Memcpy at the low* level. Should ideally use type ST/STL
-let low_memcpy (src:bytes) (dst:bytes) (h0:HS.mem{pre_cond h0 src dst}) : GTot (h1:HS.mem{post_cond h0 h1 src dst}) =
+let low_memcpy (src:buf) (dst:buf) (h0:HS.mem{pre_cond h0 src dst}) : GTot (h1:HS.mem{post_cond h0 h1 src dst}) =
   let buffers = [src; dst] in
-  let s0_heap = down_mem h0 addrs buffers in
+  let s0_heap = down_mem64 h0 addrs buffers in
   let addr1 = addrs.[(as_addr src, idx src, length src)] in
   let addr2 = addrs.[(as_addr dst, idx dst, length dst)] in
   // Not following calling conventions, but good for reduced semantics used here
   let regs = fun x -> if x = Rax then addr1 else addr2 in
   let s0 = {ok = true; regs = regs; mem = s0_heap} in
-  down_up_identity h0 addrs buffers;
+  down_up_identity64 h0 addrs buffers;
 // down_up gives us the following assertion
 //  assert (pre_v s0 src dst h0);
   let s1 = memcpy_vale s0 in
   correct_memcpy s0 src dst h0;
 // correct_memcpy gives us the following assertion
 //  assert (post_v s0 s1 src dst h0);
-  let h1 = up_mem s1.mem addrs buffers h0 in
+  let h1 = up_mem64 s1.mem addrs buffers h0 in
 // The definition of post_v gives us directly the postcondition
   h1
 
 
-// assume val memcpy_8: src:bytes -> dest:bytes ->
+// assume val memcpy_8: src:buf -> dest:buf ->
 //   STL unit 
 //   (requires (fun h -> live #UInt8.t h src /\ live #UInt8.t h dest /\ disjoint src dest 
 //     /\ length #UInt8.t src == 1 /\ length #UInt8.t dest == 1))
